theories/Abstract.v
@@ -14,23 +14,26 @@ Require Import FreeSpec.Interp.
  *)
 
 Fixpoint abstractRun
-         {S: Type}
-         {I: Type -> Type}
-         {A: Type}
-         (abs: S)
+         {S:        Type}
+         {I:        Type -> Type}
+         {A:        Type}
+         (abs:      S)
          (abs_step: forall (R:Type), I R -> R -> S -> S)
-         (int: Interp I)
-         (p: Program I A)
+         (int:      Interp I)
+         (p:        Program I A)
   : (A * (Interp I) * S) :=
   match p with
-  | ret a => (a, int, abs)
-  | instr i => (evalInstruction int i,
-                execInstruction int i,
-                abs_step _ i (evalInstruction int i) abs)
-  | bind p' f => abstractRun (snd (abstractRun abs abs_step int p'))
-                             abs_step
-                             (snd (fst (abstractRun abs abs_step int p')))
-                             (f (fst (fst (abstractRun abs abs_step int p' ))))
+  | ret a
+    => (a, int, abs)
+  | instr i
+    => (evalInstruction int i,
+        execInstruction int i,
+        abs_step _ i (evalInstruction int i) abs)
+  | bind p' f
+    => abstractRun (snd (abstractRun abs abs_step int p'))
+                   abs_step
+                   (snd (fst (abstractRun abs abs_step int p')))
+                   (f (fst (fst (abstractRun abs abs_step int p' ))))
   end.
 
 (** Similary to [FreeSpec.Program.runProgram], we define several
@@ -40,35 +43,35 @@ Fixpoint abstractRun
  *)
 
 Definition abstractExec
-           {S: Type}
-           {I: Type -> Type}
-           {A: Type}
-           (abs: S)
+           {S:        Type}
+           {I:        Type -> Type}
+           {A:        Type}
+           (abs:      S)
            (abs_step: forall (R:Type), I R -> R -> S -> S)
-           (int: Interp I)
-           (p: Program I A)
+           (int:      Interp I)
+           (p:        Program I A)
   : Interp I :=
   snd (fst (abstractRun abs abs_step int p)).
 
 Definition abstractEval
-           {S: Type}
-           {I: Type -> Type}
-           {A: Type}
-           (abs: S)
+           {S:        Type}
+           {I:        Type -> Type}
+           {A:        Type}
+           (abs:      S)
            (abs_step: forall (R:Type), I R -> R -> S -> S)
-           (int: Interp I)
-           (p: Program I A)
+           (int:      Interp I)
+           (p:        Program I A)
   : A :=
   fst (fst (abstractRun abs abs_step int p)).
 
 Definition deriveAbstraction
-           {S: Type}
-           {I: Type -> Type}
-           {A: Type}
-           (abs: S)
+           {S:        Type}
+           {I:        Type -> Type}
+           {A:        Type}
+           (abs:      S)
            (abs_step: forall (R: Type), I R -> R -> S -> S)
-           (int: Interp I)
-           (p: Program I A)
+           (int:      Interp I)
+           (p:        Program I A)
   : S :=
   snd (abstractRun abs abs_step int p).
 
@@ -85,10 +88,10 @@ Lemma abstract_run_run_program_same
       {S: Type}
       {I: Type -> Type}
       {A: Type}
-  : forall (p: Program I A)
-           (abs: S)
+  : forall (p:        Program I A)
+           (abs:      S)
            (abs_step: forall (R: Type), I R -> R -> S -> S)
-           (int: Interp I),
+           (int:      Interp I),
     fst (abstractRun abs abs_step int p) = runProgram int p.
 Proof.
   induction p; intros abs abs_step int; cbn.
@@ -101,10 +104,10 @@ Lemma abstract_eval_eval_program_same
       {S: Type}
       {I: Type -> Type}
       {A: Type}
-  : forall (p: Program I A)
-           (abs: S)
+  : forall (p:        Program I A)
+           (abs:      S)
            (abs_step: forall (R: Type), I R -> R -> S -> S)
-           (int: Interp I),
+           (int:      Interp I),
     abstractEval abs abs_step int p = evalProgram int p.
 Proof.
   intros p abs abs_step int.
@@ -117,10 +120,10 @@ Lemma abstract_exec_exec_program_same
       {S: Type}
       {I: Type -> Type}
       {A: Type}
-  : forall (p: Program I A)
-           (abs: S)
+  : forall (p:        Program I A)
+           (abs:      S)
            (abs_step: forall (R: Type), I R -> R -> S -> S)
-           (int: Interp I),
+           (int:      Interp I),
     abstractExec abs abs_step int p = execProgram int p.
 Proof.
   intros p abs abs_step int.
