theories/Refine.v
@@ -16,11 +16,11 @@ Definition StatefulRefinement
     Ii A -> S -> Program Io (A * S).
 
 Definition StatefulInterpret
-           {Ii: Type -> Type}
-           {Io: Type -> Type}
-           {S:  Type}
-           (sr: StatefulRefinement Ii Io S)
-           (s: S)
+           {Ii:  Type -> Type}
+           {Io:  Type -> Type}
+           {S:   Type}
+           (sr:  StatefulRefinement Ii Io S)
+           (s:   S)
            (int: Interp Io)
   : Interp Ii :=
     mkInterp (fun {A: Type}
@@ -44,37 +44,37 @@ Definition sync_pred
   := Si -> S -> So -> Type.
 
 Definition compliant_refinement
-           {Si So: Type}
-           {Ii Io: Interface}
-           {S: Type}
-           (sr: StatefulRefinement Ii Io S)
+           {Si So:  Type}
+           {Ii Io:  Interface}
+           {S:      Type}
+           (sr:     StatefulRefinement Ii Io S)
            (master: Contract Si Ii)
-           (slave: Contract So Io)
-           (sync: sync_pred Si So S) :=
+           (slave:  Contract So Io)
+           (sync:   sync_pred Si So S) :=
   forall (si: Si)
-         (s: S)
+         (s:  S)
          (so: So)
-         {A: Type}
-         (i: Ii A),
+         {A:  Type}
+         (i:  Ii A),
     sync si s so
     -> requirements master i si
     -> (sr A i s) :> slave[so].
 
 Definition sync_preservation
-           {Si So: Type}
-           {Ii Io: Interface}
-           {S: Type}
-           (sr: StatefulRefinement Ii Io S)
+           {Si So:  Type}
+           {Ii Io:  Interface}
+           {S:      Type}
+           (sr:     StatefulRefinement Ii Io S)
            (master: Contract Si Ii)
-           (slave: Contract So Io)
-           (sync: sync_pred Si So S) :=
-  forall (si: Si)
-         (s: S)
-         (so: So)
-         (int: Interp Io)
+           (slave:  Contract So Io)
+           (sync:   sync_pred Si So S) :=
+  forall (si:   Si)
+         (s:    S)
+         (so:   So)
+         (int:  Interp Io)
          (Henf: int :> slave[so])
-         {A: Type}
-         (i: Ii A),
+         {A:    Type}
+         (i:    Ii A),
   sync si s so
   -> requirements master i si
   -> sync (abstract_step master i (fst (evalProgram int (sr A i s))) si)
@@ -82,49 +82,50 @@ Definition sync_preservation
           (contract_derive (sr A i s) int slave so).
 
 Definition sync_promises
-           {Si So: Type}
-           {Ii Io: Interface}
-           {S: Type}
-           (sr: StatefulRefinement Ii Io S)
+           {Si So:  Type}
+           {Ii Io:  Interface}
+           {S:      Type}
+           (sr:     StatefulRefinement Ii Io S)
            (master: Contract Si Ii)
-           (slave: Contract So Io)
-           (sync: sync_pred Si So S) :=
-  forall (si: Si)
-         (s: S)
-         (so: So)
-         (int: Interp Io)
+           (slave:  Contract So Io)
+           (sync:   sync_pred Si So S) :=
+  forall (si:   Si)
+         (s:    S)
+         (so:   So)
+         (int:  Interp Io)
          (Henf: int :> slave[so])
-         {A: Type}
-         (i: Ii A),
+         {A:    Type}
+         (i:    Ii A),
   sync si s so
   -> requirements master i si
   -> promises master i (fst (evalProgram int (sr A i s))) si.
 
 Theorem enforcer_refinement
-        {Si So: Type}
-        {Ii Io: Interface}
-        {S: Type}
-        (sr: StatefulRefinement Ii Io S)
-        (master: Contract Si Ii)
-        (slave: Contract So Io)
-        (sync: sync_pred Si So S)
-        (Hsyncpres: sync_preservation sr master slave sync)
-        (Hsyncp: sync_promises sr master slave sync)
+        {Si So:      Type}
+        {Ii Io:      Interface}
+        {S:          Type}
+        (sr:         StatefulRefinement Ii Io S)
+        (master:     Contract Si Ii)
+        (slave:      Contract So Io)
+        (sync:       sync_pred Si So S)
+        (Hsyncpres:  sync_preservation sr master slave sync)
+        (Hsyncp:     sync_promises sr master slave sync)
         (Hcompliant: compliant_refinement sr master slave sync)
-  : forall (si: Si)
-           (s: S)
-           (so: So)
-           (int: Interp Io)
+  : forall (si:   Si)
+           (s:    S)
+           (so:   So)
+           (int:  Interp Io)
            (Henf: int :> slave[so]),
     sync si s so
-    -> (StatefulInterpret sr s int) :> master[si].
+    -> StatefulInterpret sr s int :> master[si].
 Proof.
   cofix.
   intros si s so int Henf Hsync.
   constructor.
   + intros A i Hreq.
     unfold sync_promises in Hsyncp.
-    assert (evalInstruction (StatefulInterpret sr s int) i = fst (evalProgram int (sr A i s)))
+    assert (evalInstruction (StatefulInterpret sr s int) i
+            = fst (evalProgram int (sr A i s)))
       as Heq by reflexivity.
     rewrite Heq.
     apply (Hsyncp si s so int Henf A i Hsync Hreq).
